theories/ListSelector.v
@@ -1,0 +1,28 @@
+From Coq Require Import
+  List.
+Import ListNotations.
+
+Section defn.
+  Context {A : Type}.
+
+  Inductive Pick : list A -> (A * list A) -> Prop :=
+  | pick_this : forall a l,
+      Pick (a :: l) (a, l)
+  | pick_next : forall a b l l',
+      Pick l (a, l') ->
+      Pick (b :: l) (a, b :: l').
+End defn.
+
+Section tests.
+  Goal forall a,
+      Pick [1; 2] a ->
+      a = (1, [2]) \/ a = (2, [1]).
+  Proof.
+    intros a H.
+    inversion_clear H.
+    - now left.
+    - inversion_clear H0.
+      + now right.
+      + inversion H.
+  Qed.
+End tests.
